early proofwork

translation/Translator.v
@@ -1,5 +1,5 @@
 Set Implicit Arguments.
-From fiat2 Require Import Language TypeSystem.
+From fiat2 Require Import Language TypeSystem TypeSound.
 
 Require Import coqutil.Map.Interface coqutil.Datatypes.dlist.
 From Utils Require Import Utils.
@@ -29,7 +29,7 @@ Fixpoint lookup_ind {T} (name: string) (rec: list (string * T)) :=
   match rec with
   | (name', _) :: rec' => if (name' =? name) then (Success 0) else 
       n <- lookup_ind name rec' ;; Success (S n)
-  | nil => error:("var" name "not found in env")
+| nil => error:("var" name "not found in env")
   end.
 
 (*
@@ -59,7 +59,7 @@ Fixpoint pyro_env_hd (G: term) :=
   | _ => error:(G "is not an env")
   end.
 Fixpoint pyro_env_wkn (G: term) :=
-  match G with 
+match G with 
   | con "ext" [a;G'] => Success G'
   | con "emp" [] => error:(G "is empty")
   | _ => error:(G "is not an env")
@@ -71,33 +71,43 @@ Compute map.mk string type.
 Require coqutil.Map.SortedListString.
 Local Existing Instance SortedListString.map.
 
+Print map.put.
 Fixpoint fiat_env_to_map (G: list (string * type)) :=
+  match G with
+  | nil => Success map.empty
+  | (n,t)::G' => 
+      Gm <- fiat_env_to_map G' ;; 
+      match map.get Gm n with None => Success (map.put Gm n t) | Some _ => error:("key" n "already in" G) end
+  end.
+
+(*
   fold_right 
     (fun x a => map.put a (fst x) (snd x))
     map.empty G.
+ *)
 
-Compute synthesize_expr (fiat_env_to_map [("a",TBool)]) _ (EAtom (ABool true)).
+Compute fenv <- fiat_env_to_map [("a",TBool)] ;; synthesize_expr fenv _ (EAtom (ABool true)).
 
-
-(* represents the kth term in Gp. 
-wkn returns w and Gp', with w a substitution sending Gp to Gp' *)
-Definition get_ind (n: nat) (Gp: term): result term :=
-  let wkn := (fix wkn (n: nat) (Gp: term) :=
+(* wkn returns w and Gp', with w a substitution sending Gp to Gp'. essentially weakens n times *)
+Fixpoint get_ind_wkn (n: nat) (Gp: term): result (term * term) :=
     match Gp with con "ext" [A;Gp'] =>
     match n with
     | 0 => Success (con "wkn" [A;Gp'], Gp')
     | S n => 
-        '(w, Gp'') <- wkn n Gp' ;;
+        '(w, Gp'') <- get_ind_wkn n Gp' ;;
          Success ((con "cmp" [w; con "wkn" [A;Gp']; Gp''; Gp'; Gp]), Gp'')
     end
     | _ => error:(Gp "not a nonempty env")
-    end) in
+    end.
+
+(* represents the kth term in Gp. *)
+Definition get_ind (n: nat) (Gp: term): result term :=
     match n with
     | 0 => match Gp with 
       | con "ext" [A;Gp'] => Success (con "hd" [A;Gp'])
       | _ => error:(Gp "not a nonempty env")
      end
-    | S n => '(w, Gp') <- wkn n Gp ;; 
+    | S n => '(w, Gp') <- get_ind_wkn n Gp ;; 
         match Gp' with 
         | con "ext" [A';Gp''] => 
          Success (con "val_subst" [con "hd" [A';Gp'']; A'; w; Gp'; Gp])
@@ -110,40 +120,60 @@ Compute get_ind 0 x.
 Print dlist.dlist.
 Print Result.
 
-Fixpoint ty_fiat_to_pyro (ft: type) (G: list (string * type)): term :=
+Require Import FunInd.
+
+Fixpoint ty_fiat_to_pyro (ft: type): result term :=
   match ft with
-  | TBool => con "bool" []
-  | TList t => con "list" [ty_fiat_to_pyro t G]
-  | TRecord l => con "Trecord" [(
-      fold_right 
-      (fun x a => (con "cons_list_ty" [a; (ty_fiat_to_pyro (snd x) G)])) 
-      (con "empty_list_ty" []) l
-  )]
-  | _ => {{e#""}} (*TODO*)
+  | TBool => Success {{e#"bool"}}
+  | TList t => tl <- ty_fiat_to_pyro t ;; Success (con "list" [tl])
+  | TRecord l => (rec_list <- (fold_right 
+      (fun x a' => a <- a' ;; 
+      trec <- ty_fiat_to_pyro (snd x) ;; 
+      Success (con "cons_list_ty" [a; trec])) 
+      (Success {{e#"empty_list_ty"}}) l) ;; Success (con "Trecord" [rec_list]))
+  | _ => error:("fiat type" ft "not supported")
   end.
 
-Definition env_fiat_to_pyro (G: list (string * type)): term :=
+Definition term_to_sort (pt: term) :=
+  match pt with
+  | con x y => scon x y
+  | _ => scon "" []
+  end.
+
+Fixpoint env_fiat_to_pyro (G: list (string * type)): result term :=
+  match G with
+  | [] => Success {{e#"emp"}}
+  | (_,x)::G' => 
+      A <- ty_fiat_to_pyro x ;;
+      Gp <- env_fiat_to_pyro G' ;;
+      Success (con "ext" [A;Gp])
+  end.
+  (*
   fold_right 
       (fun x Gp => (con "ext" [(ty_fiat_to_pyro (snd x) G); Gp])) 
       {{e#"emp"}} G.
+   *)
 
 Compute env_fiat_to_pyro [("a", TBool); ("b", TRecord([("a",TBool)]))].
 
 Definition get_fiat_type (e: expr) (G: list (string * type)): result type :=
-  '(t,_) <- synthesize_expr map.empty (fiat_env_to_map G) e ;; Success t.
+  fenv <- fiat_env_to_map G ;;
+  '(t,_) <- synthesize_expr map.empty fenv e ;; Success t.
 
 Fixpoint expr_fiat_to_pyro (fe: expr) (G: list (string * type)): result term :=
   (*(G: tenv) (fe: expr) (ft: type) (fwt: type_of G G fe ft) := *)
-  let Gp := (env_fiat_to_pyro G) in 
+  Gp <- env_fiat_to_pyro G ;;
   match fe with
   | EVar name => n <- lookup_ind name G ;; get_ind n Gp
-  | EAtom fa => match fa with 
+| EAtom fa => match fa with 
                 | ABool b => match b with
                              | true => Success (con "true" [Gp])
                              | false => Success (con "false" [Gp])
                              end
                 | ANil sft => match sft with 
-                              | Some ft => Success (con "lempty" [ty_fiat_to_pyro ft G; Gp])
+                              | Some ft => 
+                                  A <- ty_fiat_to_pyro ft ;;
+                                  Success (con "lempty" [A; Gp])
                               | None => error:("anil defined without type")
                               end
                 | _ => error:("atom" fa "not defined yet")
@@ -159,7 +189,7 @@ Fixpoint expr_fiat_to_pyro (fe: expr) (G: list (string * type)): result term :=
       e1 <- expr_fiat_to_pyro fe1 G ;; 
       e2 <- expr_fiat_to_pyro fe2 G ;;
       ty <- get_fiat_type fe1 G ;;
-      let A := ty_fiat_to_pyro ty G in
+      A <- ty_fiat_to_pyro ty ;;
                              match op with
                              | OAnd => Success (con "andb" [e2;e1;Gp])
                              | OOr => Success (con "orb" [e2;e1;Gp])
@@ -171,13 +201,13 @@ Fixpoint expr_fiat_to_pyro (fe: expr) (G: list (string * type)): result term :=
       e1 <- expr_fiat_to_pyro fe1 G ;;
       e2 <- expr_fiat_to_pyro fe2 G ;;
       ty <- get_fiat_type fe1 G ;;
-      let A := ty_fiat_to_pyro ty G in
+      A <- ty_fiat_to_pyro ty ;;
       Success (con "if" [e2;e1;A;cond;Gp])
   | ELet fe1 name fe2 => 
       ty_e1 <- get_fiat_type fe1 G ;;
       e1 <- expr_fiat_to_pyro fe1 G ;; 
       e2 <- expr_fiat_to_pyro fe2 ((name,ty_e1)::G) ;; 
-      let A := ty_fiat_to_pyro ty_e1 G in
+      A <- ty_fiat_to_pyro ty_e1 ;;
       Success (con "val_subst" [
         e2;
         A;
@@ -192,7 +222,7 @@ Fixpoint expr_fiat_to_pyro (fe: expr) (G: list (string * type)): result term :=
         | (name, expr) :: gl' => 
             v <- expr_fiat_to_pyro expr G ;;
             ty <- get_fiat_type expr G ;;
-            let A := ty_fiat_to_pyro ty G in
+            A <- ty_fiat_to_pyro ty ;;
             '(l, lty) <- build_rec gl' Gp ;;
             Success (con "cons_record" [l;v;lty;A;Gp], con "cons_list_ty" [lty;A])
         end
@@ -232,18 +262,35 @@ Compute trx.
 (* synthesize type in typesystem.v? *)
 Compute lang.
 
-(*
+Ltac t'' := repeat (
+  match goal with
+  | [|-Model.wf_term _ _ _] => t'
+  | [|-wf_term _ _ _ _] => eapply wf_term_by'
+  | [|-wf_args _ _ _] => econstructor
+  | [|-_] => unshelve (repeat t); simpl
+  end).
+
+Derive te
+  SuchThat (elab_term (value_subst) [] {{e#"emp"}} te {{s#"env"}} )
+  As te_wf.
+Proof.  t''.  Qed.
+Print te. Print te_wf.
+
+Print wf_term.
+
+Goal wf_term (value_subst) [] {{e#"emp"}} {{s#"env"}}.
+Proof.  t''.  Qed.
+
 Derive trx_derived
-  SuchThat (elab_term (fiat++value_subst) [] {{e#"false"}} trx_derived {{s#"val" #"emp" #"bool"}} )
+  SuchThat (elab_term (fiat++value_subst++exp_subst) [] {{e#"cons" #"false" (#"lempty" #"bool")}} trx_derived {{s#"val" #"emp" (#"list" #"bool")}} )
   As trx_wf.
-Proof.
-  unfold trx, trx_derived.
-  unshelve (repeat t); apply todo.
-Qed.
+Proof. t''. Qed.
+Print trx_derived.  Print trx_wf.
+
+Goal wf_term (fiat++value_subst++exp_subst) [] {{e#"true" #"emp"}} {{s#"val" #"emp" #"bool"}}.
+Proof.  t''.  Qed.
 
 Compute trx_derived.
-Goal (trx = Success trx_derived). Proof. auto. Qed.
-*)
 
 Definition trx' := match (
   expr_fiat_to_pyro (
@@ -252,19 +299,17 @@ Definition trx' := match (
     ELet (EAtom (ABool true)) "y" (
       EBinop OAnd (EVar "x") (EVar "y")))
    *)
-  (*
-  ELet (EAtom (ABool false)) "x" (
-   *)
   ELet (EAtom (ABool false)) "x" (
   ELet (EAtom (ABool true)) "y" (
-   EUnop ONot (EVar "x")))
+   EUnop ONot (EVar "y")))
   ) [])
   with Success x => x | _ => {{e#""}} end.
 
-Compute trx'.
+Goal wf_term (fiat++value_subst++exp_subst) [] trx' {{s#"val" #"emp" #"bool"}}.
+Proof.  t''.  Qed.
+
 Compute hide_term_implicits (fiat++value_subst++exp_subst) trx'.
 
-(*
 Compute hide_term_implicits (fiat++value_subst++exp_subst)
   (PositiveInstantiation.egraph_simpl' (fiat++value_subst++exp_subst) 20 20 60 [] trx').
 
@@ -273,25 +318,21 @@ Compute hide_term_implicits (fiat++value_subst++exp_subst)
 (* synthesize type in typesystem.v? *)
 Compute lang.
 
-Derive trx_derived
-  SuchThat (elab_term (fiat++value_subst) [] trx trx_derived {{s#"val" #"emp" #"bool"}} )
-  As trx_wf.
-Proof.
-  unfold trx, trx_derived.
-  unshelve (repeat t); apply todo.
-Qed.
-Compute trx_derived.
- *)
-
 (*Compute hide_term_implicits (fiat++value_subst)
    (PositiveInstantiation.egraph_simpl' (fiat++value_subst) 5 5 5 [] trx_derived).*)
 
-Compute 
-  tr <- expr_fiat_to_pyro 
-    (ERecord [("a", EAtom (ABool true)); ("b", EAtom (ABool false))]) nil ;;
-  Success (hide_term_implicits (fiat++value_subst++exp_subst) tr).
+Definition tr :=
+  match expr_fiat_to_pyro 
+    (ERecord [("a", EAtom (ABool true)); ("b", EAtom (ABool false))]) nil 
+    with Success x => x | _ => {{e#""}} end.
+Compute tr.
+Goal wf_term (fiat++value_subst++exp_subst) [] tr {{s#"val" #"emp" (#"Trecord" (#"cons_list_ty" #"bool" (#"cons_list_ty" #"bool" #"empty_list_ty")))}}.
+Proof. t''. Qed.
+  
+    (*;;
+       Success (hide_term_implicits (fiat++value_subst++exp_subst) tr).*)
 
-Compute ty_fiat_to_pyro (TRecord [("a", TBool); ("b", TBool)]) nil.
+Compute ty_fiat_to_pyro (TRecord [("a", TBool); ("b", TBool)]).
 Compute expr_fiat_to_pyro (EAtom (ABool true)) nil.
 (* Success {{e#"true"}} *)
 Compute expr_fiat_to_pyro (EUnop ONot (EAtom (ABool true))) nil.
@@ -305,20 +346,6 @@ tr <- expr_fiat_to_pyro (
       (EAtom (ANil (Some (TRecord [("a", TBool); ("b", TBool)]))))
     )
   )
-) nil ;;
-  Success (hide_term_implicits (fiat++value_subst++exp_subst) tr).
-
-Compute tr <- expr_fiat_to_pyro (EFilter 
-  LikeList 
-  (EBinop OCons 
-    (ERecord [("a", EAtom (ABool true)); ("b", EAtom (ABool false))])
-    (EBinop OCons
-      (ERecord [("a", EAtom (ABool false)); ("b", EAtom (ABool false))])
-      (EAtom (ANil (Some(TRecord [("a", TBool); ("b", TBool)]))))
-    )
-  )
-  "r"
-  (EAccess (EVar "r") "a")  
 ) nil ;;
   Success (hide_term_implicits (fiat++value_subst++exp_subst) tr).
 
@@ -401,4 +428,365 @@ Compute pytx.
 Compute expr_pyro_to_fiat pytx.
 Goal (Success tx) = (expr_pyro_to_fiat pytx). Proof. auto. Qed.
 
-Compute (PositiveInstantiation.egraph_simpl' (fiat++value_subst++exp_subst) 20 20 60 [] pytx).
+Search type_of.
+Ltac inj_all := repeat (try case_match;
+  match goal with
+  | [H: (Success ?a) = (Success ?b) |- _] => injection H as H
+  | [H: (Some ?a) = (Some ?b) |- _] => injection H as H
+  | [H: ?a =? ?b = true |-_] => try rewrite String.eqb_eq in H
+  | [H: ?a =? ?b = false |-_] => try rewrite String.eqb_neq in H
+  | [H: ?a = ?a |-_] => clear H
+  | [H: ?b = Success ?a |- _] => symmetry in H
+  | [|- _] => idtac
+  end; simpl in *; subst; try discriminate; auto).
+
+Ltac invert_type_of := repeat (
+  match goal with
+  | [H: type_of_atom _ _ |-_] => inversion H; clear H
+  | [H: type_of_unop _ _ _ |-_] => inversion H; clear H
+  | [H: type_of_binop _ _ _ _ |-_] => inversion H; clear H
+  | [H: type_of_ternop _ _ _ _ _ |-_] => inversion H; clear H
+  end; subst; try discriminate).
+
+Search "get".
+Ltac map_simpl := repeat (match goal with
+  | [H: map.get (map.put ?m ?k ?v) ?k = _ |-_] => erewrite map.get_put_same in H
+  | [H: map.get (map.put ?m ?k ?v) ?k' = _, H': ?k <> ?k' |-_] => (erewrite map.get_put_diff in H; auto)
+  | [H: map.get (map.put ?m ?k ?v) ?k' = _, H': ?k' <> ?k |-_] => (erewrite map.get_put_diff in H; auto)
+end).
+
+
+
+Opaque fiat value_subst exp_subst.
+
+Search type_wf.
+
+(*
+Check type_wf_ind.
+Theorem type_ind_full {P}:
+  P TWord -> P TInt -> P TBool -> P TString -> P TUnit ->
+  (forall t : type, P t -> P (TOption t)) ->
+  (forall t : type, P t -> P (TList t)) ->
+  (forall l : list (string * type),
+                NoDup (map fst l) ->
+                StronglySorted
+                  (fun p p' : string * type =>
+                   is_true (Value.record_entry_leb p p'))
+                  l ->
+                  Forall P (map snd l) -> P (TRecord l)) ->
+  (forall kt vt : type,
+  P kt -> P vt -> P (TDict kt vt)) ->
+  (forall t : type, P t -> P (TBag t)) ->
+  (forall t : type, P t -> P(TSet t)) ->
+  forall t, type_wf t -> P t.
+Proof.
+  intros. induction H10; eauto.
+  induction l.
+
+Print type_wf.
+ *)
+
+Definition fenv_wf (Genv: list(string*type)) :=
+  exists fenv (HGenv: Success fenv = fiat_env_to_map Genv),
+  tenv_wf fenv.
+Hint Unfold fenv_wf.
+
+Theorem ty_fiat_to_pyro_wf:
+  forall ft
+  (Htwf: type_wf ft),
+  forall A
+  (Hty: Success A = ty_fiat_to_pyro ft),
+  wf_term (fiat++value_subst++exp_subst) [] A {{s#"ty"}}.
+
+Proof.
+  intros ft _.
+  induction ft using type_IH;
+  intros; inj_all; t''; eauto. 
+  generalize dependent a.
+  induction l; intros; repeat (inj_all; t'');
+  inversion H; eauto.
+Qed.
+Hint Resolve ty_fiat_to_pyro_wf: core.
+
+Opaque map.put map.get.
+Axiom fenv_map_ok: map.ok (SortedListString.map type). (*TODO*)
+Hint Resolve fenv_map_ok.
+
+Theorem fiat_env_to_map_contains {x}{t}{Genv}{G}:
+  Success G = fiat_env_to_map ((x,t)::Genv) ->
+  tenv_wf G -> map.get G x = Some t.
+Proof. 
+  simpl; intros; repeat (case_match; try discriminate).
+  inversion H.
+  eapply map.get_put_same. Unshelve. eauto.
+Qed.
+
+Theorem string_eq_destruct (x:string) (x':string):
+  (x=x' \/ x<>x').
+Proof.
+  rewrite <- String.eqb_neq;
+  rewrite <- String.eqb_eq.
+  destruct (x=?x'); eauto.
+Qed.
+
+Theorem fiat_env_to_map_contents {x}{t}{Genv}{G}{G'}:
+  Success G = fiat_env_to_map ((x,t)::Genv) ->
+  Success G' = fiat_env_to_map (Genv) ->
+  tenv_wf G -> 
+  forall x' t', map.get G x' = Some t' ->
+  (x=x' /\ t=t') \/ (map.get G' x' = Some t').
+Proof.
+  pose fenv_map_ok.
+  simpl; intros; repeat (case_match; try discriminate).
+  injection H0 as H0; rewrite <- H0 in *; clear H0 a.
+  injection H as H; rewrite H in *; clear H G.
+  destruct (string_eq_destruct x' x).
+  - left; inj_all; map_simpl. inj_all.
+  - right; map_simpl.
+Qed.
+
+Theorem fenv_wf_ext {G} {s} {t}:
+  fenv_wf ((s,t)::G) -> fenv_wf G.
+Proof.
+  pose fenv_map_ok.
+  intros. destruct H as [fenv [H H']]. inj_all.
+  econstructor; eexists; eauto.
+  unfold tenv_wf in *; intros.
+  eapply H' with x0; erewrite map.get_put_diff; eauto.
+  unfold "<>"; intros; subst. rewrite H in *; discriminate.
+Qed.
+
+Theorem fenv_wf__type_wf {G} {s} {t}:
+  fenv_wf ((s,t)::G) -> type_wf t.
+Proof.
+  intros. destruct H as [fenv [H H']]. inj_all.
+  eapply H' with s; eauto using map.get_put_same.
+Qed.
+
+Hint Resolve fiat_env_to_map_contains fiat_env_to_map_contents fenv_wf_ext fenv_wf__type_wf: core.
+
+Ltac wf_term_ty := 
+  lazymatch goal with
+  | [H: Success ?a = ty_fiat_to_pyro ?ft ?Genv |- (wf_term _ _ ?a {{s #"ty"}})] => 
+    eapply ty_fiat_to_pyro_wf; try apply H; auto
+  end.
+
+Theorem env_fiat_to_pyro_wf:
+  forall Genv
+  (HGenv: fenv_wf Genv),
+  forall Gp (Henv: Success Gp = env_fiat_to_pyro Genv),
+  wf_term (fiat++value_subst++exp_subst) [] Gp {{s#"env"}}.
+Proof.
+  induction Genv as [|(n,t)]; 
+  intros; simpl in Henv; try solve [inversion Henv; t''].
+  inj_all. t''; eauto.
+Qed.
+Hint Resolve env_fiat_to_pyro_wf: core.
+
+Theorem env_fiat_to_pyro_contents_wf:
+  forall Genv
+  (HGenv: fenv_wf Genv),
+  forall G A (Henv: Success (con "ext" [A;G]) = env_fiat_to_pyro Genv),
+  wf_term (fiat++value_subst++exp_subst) [] A {{s#"ty"}} /\
+  wf_term (fiat++value_subst++exp_subst) [] G {{s#"env"}}.
+Proof.
+  induction Genv as [|(n,t)]; intros; inj_all.
+  apply conj; eauto.
+Qed.
+
+Hint Resolve env_fiat_to_pyro_contents_wf type_of__type_wf: core.
+
+Theorem get_ind_wkn_fiat_to_pyro_wf (n:nat):
+  forall Genv (HGenv: fenv_wf Genv) 
+  Gp (Henv: Success Gp = env_fiat_to_pyro Genv),
+  forall wkn Gp'
+  (Hw: Success (wkn, Gp') = get_ind_wkn n Gp),
+  wf_term (fiat++value_subst++exp_subst) [] Gp' {{s#"env"}} /\
+  wf_term (fiat++value_subst++exp_subst) [] wkn (scon "sub" [Gp';Gp]) /\
+  (forall A Gp'', con "ext" [A;Gp''] = Gp' -> 
+  wf_term (fiat++value_subst++exp_subst) [] Gp'' {{s#"env"}} /\
+  wf_term (fiat++value_subst++exp_subst) [] A {{s#"ty"}} /\
+  forall {d}, Success A = ty_fiat_to_pyro (snd (nth (S n) Genv d))).
+Proof.
+  induction n; intros; destruct Genv; inj_all.
+  - repeat (try apply conj); t''; eauto.
+    intros. destruct Genv; inj_all. repeat (try apply conj); eauto.
+  - edestruct IHn with (Genv:=Genv) as [H [H' H'']]; eauto.
+    repeat (try apply conj); t''; eauto.
+Qed.
+Hint Resolve get_ind_wkn_fiat_to_pyro_wf: core.
+
+Theorem get_ind_fiat_to_pyro_wf (n:nat):
+  forall Genv (HGenv: fenv_wf Genv) 
+  Gp (Henv: Success Gp = env_fiat_to_pyro Genv),
+  forall A {d} (Hty: Success A = ty_fiat_to_pyro (snd (nth n Genv d))),
+  forall pt
+  (Hw: Success pt = get_ind n Gp),
+  wf_term (fiat++value_subst++exp_subst) [] pt (scon "val" [A;Gp]).
+Proof.
+  destruct n.
+  - intros. destruct Genv; inj_all. t''; eauto.
+  - destruct n.
+    + intros. 
+      pose proof get_ind_wkn_fiat_to_pyro_wf 0 HGenv Henv as H'.
+      destruct Genv; inj_all; destruct Genv; inj_all; 
+      eauto.
+      edestruct H'; eauto. clear H'.
+      destruct H0 as [Hswf Hext].
+      edestruct Hext; eauto; clear Hext.
+      t''; eauto.
+    + intros. 
+      destruct Genv; inj_all.
+      assert (HGenv': fenv_wf Genv) by eauto.
+      pose proof get_ind_wkn_fiat_to_pyro_wf n HGenv' as H''.
+      destruct Genv; inj_all. { destruct n; inj_all. }
+      eauto.
+      edestruct H''; eauto. clear H''.
+      destruct H0 as [Hswf Hext].
+      edestruct Hext as [HGp'' [Ha Hn]]; eauto; clear Hext.
+      specialize Hn with d; rewrite <- Hn in Hty; inj_all.
+      t''; eauto.
+Qed.
+Hint Resolve get_ind_fiat_to_pyro_wf: core.
+
+Theorem type_lookup:
+  forall a x Gstore Genv {fstore} {fenv}
+  (HGst: Success fstore = fiat_env_to_map Gstore) 
+  (HFst: fenv_wf Gstore)
+  (HGenv: Success fenv = fiat_env_to_map Genv) 
+  (HFenv: fenv_wf Genv)
+  (Hlookup: Success a = lookup_ind x Genv) {d},
+  type_of fstore fenv (EVar x) (snd (nth a Genv d)).
+Proof.
+  pose fenv_map_ok.
+  induction a; intros; destruct Genv; inj_all.
+  - econstructor; eauto using map.get_put_same.
+  - econstructor; erewrite map.get_put_diff; eauto.
+    assert (H: type_of fstore a (EVar x0) (snd (nth a0 Genv d))) by eauto.
+    inversion H; eauto.
+Qed.
+Hint Resolve type_lookup: core.
+
+Search synthesize_expr.
+
+Theorem fiat_type_sound:
+  forall Gstore Genv {fstore} {fenv} fe ft
+  (HGst: Success fstore = fiat_env_to_map Gstore) 
+  (HFst: fenv_wf Gstore)
+  (HGenv: Success fenv = fiat_env_to_map Genv) 
+  (HFenv: fenv_wf Genv)
+  (Hft: Success ft = get_fiat_type fe Genv),
+  type_of fstore fenv fe ft.
+Proof.
+  pose fenv_map_ok.
+  unfold get_fiat_type.
+  intros.
+  inj_all.
+  destruct HFst as [fst [Hst Hst']];
+  destruct HFenv as [fenv' [Henv Henv']].
+  rewrite <- Hst in *.
+  rewrite <- Henv in *;
+  inj_all. symmetry in case_match_eqn0.
+  eapply proj1.
+
+  epose typechecker_sound.
+
+
+Theorem expr_fiat_to_pyro_wf:
+  forall Gstore Genv {fstore} {fenv} fe ft
+  (HGst: Success fstore = fiat_env_to_map Gstore) 
+  (HFst: fenv_wf Gstore)
+  (HGenv: Success fenv = fiat_env_to_map Genv) 
+  (HFenv: fenv_wf Genv)
+  (Hty: type_of fstore fenv fe ft),
+  forall pt A Gp
+  (He: Success pt = expr_fiat_to_pyro fe Genv)
+  (Hty: Success A = ty_fiat_to_pyro ft)
+  (Henv: Success Gp = env_fiat_to_pyro Genv),
+  wf_term (fiat++value_subst++exp_subst) [] pt (scon "val" [A;Gp]).
+Proof.
+  pose fenv_map_ok.
+  induction fe; simpl; 
+  unfold get_fiat_type in *; inj_all; intros;
+  inversion Hty; clear Hty; invert_type_of; inj_all; try solve [t''; eauto].
+  (*symmetry in case_match_eqn; 
+  pose proof env_fiat_to_pyro_wf Genv HGenv HFenv case_match_eqn as HGenv_wf.*)
+  - assert (Hty': type_of fstore fenv (EVar x0) (snd (nth a0 Genv ("",TUnit)))) by eauto. 
+    inversion Hty'. rewrite H1 in H0.
+    inj_all; eauto. (*eapply get_ind_fiat_to_pyro_wf with (Genv:=Genv)*)
+  - 
+    assert (type_of fstore fenv fe1 a2). {
+    unfold get_fiat_type in *; inj_all.
+
+
+  }
+    assert (wf_term (fiat ++ value_subst ++ exp_subst) [] a0 (scon "val" [a4;a])) by eauto.
+assert (wf_term (fiat ++ value_subst ++ exp_subst) [] a1 (scon "val" [a4;a])) by eauto.
+    eapply IHfe1 with (Gp:=a) (pt:=a0) (ft:=t1) (A:=a4).
+    t''; eauto.
+    inversion Hty.
+    inversion H0; clear H0;
+    inj_all.
+  - inversion Hty; inversion H0; inj_all. t''; eauto.
+  - inversion Hty; inversion H0; inj_all. t''; eauto.
+  - inversion Hty; inversion H0; inj_all. t''; eauto.
+  - inversion Hty; inversion H1; inj_all. t''; eauto.
+  - inversion Hty; inversion H1; inj_all.
+  - inversion Hty. inversion H1; inj_all.
+  - inversion Hty; inversion H0
+    edestruct IHfe with (ft:=TBool); eauto. {
+      inversion Hty; inversion H1; inj_all.
+    }
+    inj_all; eexists; t''; eauto.
+    assert (type_wf t)
+
+
+    destruct Genv; try discriminate.
+    generalize dependent a;
+    generalize dependent Genv;
+    generalize dependent x0.
+    destruct a0. {
+      intros; inj_all.
+      eexists. t''; eauto.
+    }
+    induction a0; intros; destruct Genv; try solve [inj_all].
+    * inj_all. eexists; t''; eauto.
+    * inj_all. eexists; t''; eauto.
+
+      pose proof tenv_wf_ext HFenv case_match_eqn4 as HFenv'.
+      pose proof tenv_wf_ext HFenv' case_match_eqn3 as HFenv''.
+      (*
+      epose proof env_fiat_to_pyro_wf Genv case_match_eqn2 HFenv'' case_match_eqn7 as H.
+      epose proof ty_fiat_to_pyro_wf _ _ HFenv' _ case_match_eqn6.
+      epose proof ty_fiat_to_pyro_wf _ _ HFenv _ case_match_eqn5.
+       *)
+
+      (*
+      destruct (string_eq_destruct x0 s). {
+        subst; assert (Ht: s=?s=true) by (rewrite String.eqb_eq; auto). simpl in case_match_eqn0; rewrite Ht in case_match_eqn0; discriminate.
+      }
+         inj_all; map_simpl.*)
+      assert (Hlookup: lookup_ind x0 ((s0,t5)::Genv) = Success (S a4)). {
+        simpl.
+        assert (Ht: s0=?x0=false) by (rewrite String.eqb_neq; auto).
+        rewrite Ht.
+        inj_all.
+      }
+      edestruct IHa0 with  (fstore:=fstore); try eapply Hlookup; try eapply HFenv'; inj_all; eauto; try solve [inversion Hty; erewrite map.get_put_diff in H0; eauto; constructor; eauto].
+      clear IHa0. 
+      assert (wf_term (fiat ++ value_subst ++ exp_subst) [] t2 {{s #"ty"}}). {
+        inversion H.
+        - 
+
+      }
+        inj_all. eexists.
+        t''; eauto.
+      all: try solve [wf_term_ty; try apply HFenv; inj_all; eauto].
+      all: try solve [wf_term_ty; try apply HFenv'; inj_all; eauto].
+      all: try solve [wf_term_ty; try apply HFenv''; inj_all; eauto].
+      { 
+
+
+      }
+      Unshelve. all: try eauto using map.get_put_same.
+    
